src/BFile.v
@@ -1138,9 +1138,9 @@ Module BFILE.
            [[[ flist ::: (Fi * inum |-> f) ]]] *
            [[[ (BFData f) ::: (Fd * off |-> vs) ]]] *
            [[ sync_invariant F ]]
-    POST:hm' RET:ms'  exists flist' f' bn ds0 ds',
+    POST:hm' RET:ms'  exists flist' f' bn ds',
            LOG.rep lxp F (LOG.ActiveTxn ds' ds'!!) (MSLL ms') hm' *
-           [[ ds' = dsupd ds0 bn (v, vsmerge vs) /\ diskset_was ds0 ds ]] *
+           [[ ds' = dsupd ds bn (v, vsmerge vs) ]] *
            [[ block_belong_to_file ilist bn inum off ]] *
            [[ MSAlloc ms = MSAlloc ms' ]] *
            (* spec about files on the latest diskset *)
@@ -1154,7 +1154,7 @@ Module BFILE.
            LOG.recover_any lxp F (dsupd ds bn (v, vsmerge vs)) hm'
     >} dwrite lxp ixp inum off v ms.
   Proof.
-    unfold dwrite, diskset_was.
+    unfold dwrite.
     prestep; norml.
     denote  (list2nmem ds !!) as Hz.
     eapply block_belong_to_file_ok in Hz as Hb; eauto.
@@ -1187,18 +1187,6 @@ Module BFILE.
     cancel.
     eauto.
     cancel.
-
-    intuition simpl.
-    2: sepauto. 2: sepauto.
-    pred_apply; cancel.
-    setoid_rewrite <- updN_selN_eq with (l := ilist) (ix := inum) at 4.
-    rewrite listmatch_updN_removeN by omega.
-    unfold file_match at 3; cancel; eauto.
-    setoid_rewrite <- updN_selN_eq with (l := INODE.IBlocks _) (ix := off) at 3.
-    erewrite map_updN by omega; filldef.
-    rewrite listmatch_updN_removeN by omega.
-    cancel.
-    eauto.
 
     repeat xcrash_rewrite.
     xform_norm; xform_normr.
